\subsection*{Review Problems Chapter 4}
\textbf{Problem 6}
The auxillary equation has roots
\begin{align*}
    r^2 + 8 r - 14
    &\implies r = \frac{-8 \pm \sqrt{64 + 56}}{2} \\
    &\implies r = -4 \pm \sqrt{30}
\end{align*}

The general solution is 
\[
    y = C_1e^{-4-\sqrt{30}} + C_2e^{-4+\sqrt{30}}
\]
\textbf{Problem 10}
The auxillary equation has roots 
\[
    r^2 + 11 = 0
    \implies r = i\sqrt{11}
\]

The general solution is 
\[
    y = C_1\cos{\sqrt{11} t} + C_2\sin{\sqrt{11} t}
\]
\textbf{Problem 13}
The auxillary equation has roots 
\[
    r^2 + 16 = 0
    \implies r = 4i
\]
The homogenous solution is
\[
    y_h = c_1\cos 4t + c_2\sin 4t
\]
The particular solution has form 
\[
    y_p = (A_1t + A_0)e^{t}
\]
Thus,
\begin{align*}
     A_1e^t(t+2)+ A_0e^t + 16e^{t}(A_1t + A_0) = te^t 
     &\implies 17A_1 = 1, 2A_1 + 17A_0 = 0 \\  
     &\implies A_1 = \frac{1}{17}, A_0 = -\frac{2}{289}  
\end{align*}
The general solution is 
\[
    y = c_1\cos 4t + c_2\sin 4t + \frac{te^t}{17} - \frac{2e^t}{289}  
\]
\textbf{Problem 20}
The auxillary equation is 
\[
    2r^2 - 1 = 0
    \implies r = \pm \frac{1}{\sqrt{2}}
\]
The homogeneous solution is 
\[
    y_h = C_1e^{\frac{t}{\sqrt{2}}} + C_2e^{-\frac{t}{\sqrt{2}}}
\]
The particular solution has form
\[
    y_p = (A_1t + A_0)\cos t + (B_1t + B_0)\sin t
\]
Thus, 
\[
    -2\cos (A_1t + A_0 -2B_0 + \sin t (2A_1 + B_1t + B_0))
    - ((A_1t + A_0)\cos t + (B_1t + B_0)\sin t)
    = t\sin t
\]
This yields $A_1 = 0$, $A_0 = -\frac{4}{9}$, $B_1 = -\frac{1}{3}$, $B_0 = 0$.
The general solution is
\[
    y = C_1e^{\frac{t}{\sqrt{2}}} + C_2e^{-\frac{t}{\sqrt{2}}} 
    -\frac{4}{9}\cos t - \frac{1}{3} t\sin t
\]
\textbf{Problem 25}
The auxillary equation has roots
\[
    4r^2-12r+9 = (2r-3)^2 
    \implies r = \frac{3}{2}
\]
The homogenous solution is 
\[
    y_h = C_1e^{\frac{3}{2}t} + C_2te^{\frac{3}{2}t}
\]
The particular solution has the form 
\[
    A_0e^{3t} + B_0e^{5t}
\]
Plugging this into the equation and solving for the coefficients yields
$A_0 = \frac{1}{9}$ and $B_0 = \frac{1}{49}$
The general solution is 
\[
    y = C_1e^{\frac{3}{2}t} + C_2te^{\frac{3}{2}t} + \frac{1}{9}e^{3t} + \frac{1}{49}e^{5t}
\]
\textbf{Problem 31}
The auxillary equation has roots 
\[
    r^2-2r+10 
    \implies r = \frac{2 \pm \sqrt{4-40}}{2}
    \implies r = 1 \pm 3i
\]
The homogenous solution has form 
\[
    y_h = C_1e^t\cos 3t + C_2e^t\sin 3t
\]
The particular solution has form 
\[
    y_p = A_0\cos 3t + B_0\sin 3t
\]
Solving out for the constants yields $A_0 = 0$ and $B_0 = -1$.
The general solution is 
\[
    y = C_1e^t\cos 3t + C_2e^t\sin 3t - \sin 3t
\]
In order for the initial values to hold, $C_1 = 2$ and $C_2 = -\frac{7}{3}$.
The solution is 
\[
    y = 2e^t\cos 3t - \frac{7}{3} e^t\sin 3t - \sin 3t
\]