\subsection{Review Problems Chapter 9}
\textbf{Problem 1}
The characteristic equation is 
\[
    (6-\lambda)(1-\lambda) + 6
    = 12 - 7\lambda + \lambda^2
    = (\lambda-3)(\lambda-4)
\]
For $\lambda_1 = 3$
\[
    A - \lambda I = \begin{bmatrix}
        3 & -3 \\
        2 & -2
    \end{bmatrix}
\]
The eigenvector is 
\[
    \begin{bmatrix}
        1 \\ 1
    \end{bmatrix}
\]
For $\lambda_2 = 4$
\[
    A -\lambda I= \begin{bmatrix}
        2 & -3 \\
        2 & -3
    \end{bmatrix}
\]
The eigenvector is 
\[
    \begin{bmatrix}
        3 \\ 2
    \end{bmatrix}
\]

The general solution is thus 
\[
   x(t) = c_1e^{3t}
   \begin{bmatrix}
       1 \\ 1
   \end{bmatrix} +
   c_2e^{4t}
   \begin{bmatrix}
       3 \\ 2
   \end{bmatrix} 
\]
\textbf{Problem 2}
The characteristic equation is 
\[
    (3-\lambda)(1-\lambda) + 10
    = 13 - 4\lambda + \lambda^2
    \implies \lambda = \frac{4 \pm \sqrt{16-52}}{2}
    \implies \lambda = 2 \pm 3i
\]
The eigenvector of $\lambda_1 = 2 + 3i$ is 
\[
    A-\lambda I = \begin{bmatrix}
        1-3i & 2 \\
        -5 & -1-3i
    \end{bmatrix}
    \implies \begin{bmatrix}
        10 & 2+6i \\
        -5 & -1-3i
    \end{bmatrix}
    \implies 
    \implies \begin{bmatrix}
        5 & 1+3i \\
        0 & 0
    \end{bmatrix}
\]
The eigenvector is 
\[
    \begin{bmatrix}
        -1-3i \\ 5
    \end{bmatrix}
\]
The general solution is 
\[
    x(t) = c_1\left\{ 
        e^{2t}\cos 3t \begin{bmatrix} -1 \\ 5 \end{bmatrix} 
        - e^{2t}\sin 3t \begin{bmatrix} -3 \\ 0 \end{bmatrix} 
    \right\} + 
    c_2\left\{ 
        e^{2t}\sin 3t \begin{bmatrix} -1 \\ 5 \end{bmatrix} 
        + e^{2t}\cos 3t \begin{bmatrix} -3 \\ 0 \end{bmatrix} 
    \right\} 
\]
\textbf{Problem 5}
The characteristic equation is 
\[
    (1-\lambda)(4-\lambda)+2
    = 6 -5\lambda + \lambda^2
    = (\lambda-2)(\lambda-3)
\]
For $\lambda = 2$,
\[
    A = \begin{bmatrix}
        -1 & -1 \\
        2 & 2
    \end{bmatrix}
\]
The eigenvector is 
\[
    \begin{bmatrix}
        1 \\ -1
    \end{bmatrix}
\]
For $\lambda = 3$,
\[
    A = \begin{bmatrix}
        -2 & -1 \\
        2 & 1
    \end{bmatrix}
\]
The eigenvector is 
\[
    \begin{bmatrix}
        1 \\ -2
    \end{bmatrix}
\]
The fundamental matrix is 
\[
    \begin{bmatrix}
        e^{2t} & e^{3t} \\
        -e^{2t} & -e^{3t}
    \end{bmatrix}
\]
\textbf{Problem 11}
The characteristic polynomial is 
\[
    -\lambda(3-\lambda) + 2
    = \lambda^2-3\lambda+2
    = (\lambda-1)(\lambda-2)
\]
For $\lambda=1$
\[
    A-\lambda I = \begin{bmatrix}
        -1 & 1 \\
        -2 & 2
    \end{bmatrix}
\]
The eigenvector is 
\[
    \begin{bmatrix}
        1 \\ 1
    \end{bmatrix}
\]
For $\lambda=2$
\[
    A-\lambda I = \begin{bmatrix}
        -2 & 1 \\
        -2 & 1
    \end{bmatrix}
\]
The eigenvector is 
\[
    \begin{bmatrix}
        1 \\ 2
    \end{bmatrix}
\]
The general solution is 
\[
    x(t) = c_1e^t
    \begin{bmatrix}
        1 \\ 1
    \end{bmatrix} +
    c_2e^{2t}
    \begin{bmatrix}
        1 \\ 2
    \end{bmatrix}
\]
Plugging in the initial values yield 
\[
    \begin{bmatrix}
        1 \\ -1
    \end{bmatrix} 
    =
    c_1
    \begin{bmatrix}
        1 \\ 1
    \end{bmatrix} +
    c_2
    \begin{bmatrix}
        1 \\ 2
    \end{bmatrix}
\]
So $c_1 = 3$ and $c_2 = -2$.
The final solution is 
\[
    x(t) = 3e^t
    \begin{bmatrix}
        1 \\ 1
    \end{bmatrix} -
    2e^{2t}
    \begin{bmatrix}
        1 \\ 2
    \end{bmatrix}
\]