\subsection*{Section 4-5}
\textbf{Problem 1}
\begin{enumerate}
    \item $5\cos t$
    \item $\cos t - e^{2t}$
    \item $4\cos +6e^{2t}$
\end{enumerate}
\textbf{Problem 4}
The roots are 
\[
    r^2 + r = 0 \implies r = -1, 0
\]
The general solution is therefore 
\[
    y = t + C_1e^{-t} + C_2
\]
\textbf{Problem 18}
The roots are 
\[
    r^2-1 = 0 \implies r=-1, 1
\]
The particular solution has form 
\[
    y_p(t) = A_1t + A_0
\]
Solving for the coefficients yields 
\[
    y_p(t) = 11t - 1
\]
The general solution is therefore
\[
    y(t) = 11t-1 + C_1e^{-t} + C_2e^t
\]
\textbf{Problem 23}
The equation is linear and the integrating factor is 
\[
    \mu = e^{-x}
\]
Multiplying both sides by the integrating factor yields 
\[
   \der{}{x} e^{-x}y = e^{-x}
   \implies e^{-x}y = -e^{-x}
   \implies y = -1
\]
The equation has root $r=1$, so the general form is 
\[
    y = Ce^t-1
\]
At $y(0) = 0$,
\[
    y = e^t-1
\]

\textbf{Problem 24}
Integrating twice yields 
\[
    y' = 3t^2 + C_1
\]
\[
    y = t^3 + C_1t + C_2
\]
At the initial values $C_1 = -1$ and $C_2 = 3$, 
\[
    y = t^3 - t + 3
\]

\textbf{Problem 25}
The roots are 
\[
    r^2 + 1 = 0 \implies r = \pm i
\]
The homogenous solution is therefore 
\[
    y_h = C_1\cos x + C_2\sin x
\]
The particular solution is in the form 
\[
    y_p = A_0e^{-x}
\]
Solving gives $A_0 = 1$ .
The general solution has form 
\[
    y = e^{-x} + C_1\cos x + C_2\sin x
\]
Solving for constants yields 
\[
    y = e^{-x} - \cos x + \sin x
\]
\textbf{Problem 28}
The roots are 
\[
    r^2 + r - 12 = 0 
    \implies (r+4)(r-3) = 0
    \implies r=-4, r=3
\]
The homogenous solution is 
\[
    y_h = C_1e^{-4t} + C_2{3t}
\]
For $r=1,2$ are not roots, so the particular solution has form 
\[
    y_p = Ae^t + Be^{2t} + \frac{1}{12}
\]
Solving for the constants gives $A=-\frac{1}{10}$ and $B=-\frac{1}{3}$
The general solution has form 
\[
    y = -\frac{1}{10}e^t - \frac{1}{6}e^{2t} + \frac{1}{12} + C_1e^{-4t} + C_2{3t}
\]
Plugging in the initial values gives 
\[
    1 = -\frac{4}{15} + C_1 + C_2
\]
\[
    3 = -\frac{13}{30} -4C_1 + 3C_2
\]
Therefore the final solution is 
\[
    y = -\frac{1}{10}e^t - \frac{1}{6}e^{2t} + \frac{1}{12} + \frac{1}{60}e^{-4t} + \frac{7}{6}{3t}
\]