\documentclass{article}

\usepackage{amsmath}
\usepackage{amssymb}
\usepackage{hyperref}
\usepackage{mathrsfs}
\usepackage{enumerate}
\usepackage{bm}
\usepackage{physics}
\usepackage{graphicx}
\setlength{\parindent}{0pt}
\usepackage[parfill]{parskip}
\usepackage[margin=1in]{geometry}

\newcommand{\cjg}[1]{\overline{#1}}
\DeclareMathOperator\Arg{Arg}

\begin{document}
\begin{center}
	\huge{\bf Math 120A: Homework 6} \\
	Merrick Qiu
\end{center}
\section*{Problem 1}
\begin{enumerate}[(a)]
	\item $u_x = -2x$, $u_{xx} = -2$ and $u_y = 2y+2$, $u_{yy} = 2$ so $u$ is harmonic since
	$u_{xx} + u_{yy} = 0$.
	\item We need $v_y = -2x$ and $v_x = -2y-2$ for Cauchy-Riemann to hold.
	Integrating $v_y$ with respect to $y$ gives us that 
	\[
		v(x,y) = -2xy + g(x)
	\]
	Differentiating by $x$ gives us 
	\[
		v_x = -2y + g'(x) = -2y-2
	\]
	which implies $g(x) = -2x+C$.
	Therefore the harmonic conjugate is $v = -2xy-2x + C$.
	\item 
	\begin{align*}
		f(z) &= y^2+2y-x^2 + i(-2xy-2x+C) \\
		&= -(x+iy)^2 - 2i(x+iy) + iC\\
		&= -z^2 - 2iz + iC
	\end{align*}
\end{enumerate}
\newpage 
\section*{Problem 2}
	\begin{align*}
		\log(1-i) &= \log(\sqrt{2}e^{i\left(-\frac{\pi}{4}+2\pi n\right)}) \\
		&= \frac{\ln(2)}{2} + i\left(-\frac{\pi}{4}+2\pi n\right)
	\end{align*}
	The principal argument is $\frac{\pi}{4}$.
	\[
		\operatorname{Log}(1-i) = \frac{\ln(2)}{2} - i\frac{\pi}{4}
	\]
\newpage 
\section*{Problem 3}
	\[
		\log(-i) = \log(e^{i\left(-\frac{\pi}{2} + 2\pi n\right)}) = i\left(-\frac{\pi}{2} + 2\pi n\right)
	\]
	\[
		(-i)^{-i} = e^{-i\log(-i)} = e^{-\frac{\pi}{2} + 2\pi n}
	\]
	The principal value is 
	\[
		(-i)^{-i} = e^{-\frac{\pi}{2}}
	\]
\newpage 
\section*{Problem 4}
	\[
		\log(i) = \log(e^{i\left(\frac{\pi}{2} + 2\pi n\right)}) = i\left(\frac{\pi}{2} + 2\pi n\right)
	\]
	\[
		(i)^{1+i} = e^{(1+i)\log(i)} = e^{(i-1)\left(\frac{\pi}{2} + 2\pi n\right)} = e^{-\left(\frac{\pi}{2} + 2\pi n\right)}e^{i\left(\frac{\pi}{2} + 2\pi n\right)} = e^{-\left(\frac{\pi}{2} + 2\pi n\right)}i
	\]
	The principal value is 
	\[
		(i)^{1+i} = e^{-\frac{\pi}{2}}i
	\]
\newpage 
\section*{Problem 5}
	\begin{align*}
		\sin\left(z+\frac{\pi}{2}\right) &= \frac{e^{i\left(z+\frac{\pi}{2}\right)}-e^{-i\left(z+\frac{\pi}{2}\right)}}{2i} \\
		&= \frac{e^{i\frac{\pi}{2}}e^{iz}-e^{-i\frac{\pi}{2}}e^{-iz}}{2i} \\
		&= \frac{e^{iz}+e^{-iz}}{2} \\
		&= \cos(z)
	\end{align*}
\newpage 



\end{document}