\newcommand{\integral}[1]{\int_{-1}^{1} #1 \,dt}
\newcommand{\brackets}[1]{\left[ #1 \right]_{-1}^{1}}
\section{Polynomial Gram-Schmidt}

For $f_0$, we have that
\[
    f_0 
    = \frac{1}{||1||}
    = \frac{1}{\sqrt{\integral{1}}} 
    = \frac{1}{\sqrt{2}}
\]

For $f_1$, we have that
\[
    t - \inner{t}{\frac{1}{\sqrt{2}}} \cdot \frac{1}{\sqrt{2}}
    = t - \integral{\frac{1}{2} t}  \\
    = t - \brackets{\frac{1}{4} t^2}\\
    = t
\]
\[
    ||t - \inner{t}{\frac{1}{\sqrt{2}}} \cdot \frac{1}{\sqrt{2}}||
    = ||t||\\
    = \sqrt{\integral{t^2}}\\
    = \sqrt{\brackets{\frac{1}{3} t^3}}\\
    = \sqrt{\frac{2}{3}}
\]
\[
    f_1
    = \frac{t - \inner{t}{\frac{1}{2}} \cdot \frac{1}{2}}{||t - \inner{t}{\frac{1}{2}} \cdot \frac{1}{2}||}
    = \frac{t}{\sqrt{\frac{2}{3}}}
    = \sqrt{\frac{3}{2}}t
\]

For $f_2$ we have that
\begin{align*}
    t^2 - \inner{t^2}{\sqrt{\frac{3}{2}}t} \cdot \sqrt{\frac{3}{2}}t - \inner{t^2}{\frac{1}{\sqrt{2}}} \cdot \frac{1}{\sqrt{2}}
    &= t^2 - \integral{\frac{3}{2}t^3} \cdot t - \integral{\frac{1}{2}t^2}\\
    &= t^2 - \brackets{\frac{3}{8}t^4} \cdot t - \brackets{\frac{1}{6}t^3}\\
    &= t^2 - \frac{1}{3}
\end{align*}
\begin{align*}
    ||t^2 - \inner{t^2}{\sqrt{\frac{3}{2}}t} \cdot \sqrt{\frac{3}{2}}t - \inner{t^2}{\frac{1}{\sqrt{2}}} \cdot \frac{1}{\sqrt{2}}||
    &= ||t^2 - \frac{1}{3}||\\
    &= \sqrt{\integral{t^4 - \frac{2}{3}t^2 + \frac{1}{9}}}\\
    &= \sqrt{\brackets{\frac{1}{5}t^5 - \frac{2}{9}t^3 + \frac{1}{9}t}}\\
    &= \sqrt{\frac{8}{45}}
\end{align*}
\[
    f_2 
    = \frac{t^2 - \inner{t^2}{\sqrt{\frac{3}{2}}t} \cdot \sqrt{\frac{3}{2}}t - \inner{t^2}{\frac{1}{\sqrt{2}}} \cdot \frac{1}{\sqrt{2}}}{||t^2 - \inner{t^2}{\sqrt{\frac{3}{2}}t} \cdot \sqrt{\frac{3}{2}}t - \inner{t^2}{\frac{1}{\sqrt{2}}} \cdot \frac{1}{\sqrt{2}}||}
    = \frac{t^2 - \frac{1}{3}}{\sqrt{\frac{8}{45}}}
    = \sqrt{\frac{45}{8}}(t^2 - \frac{1}{3})
\]

For $f_3$ we have that
\begin{align*}
    t^3 - \inner{t^3}{\sqrt{\frac{45}{8}}(t^2 - \frac{1}{3})} \cdot \sqrt{\frac{45}{8}}(t^2 - \frac{1}{3}) &- \inner{t^3}{\sqrt{\frac{3}{2}}t} \cdot \sqrt{\frac{3}{2}}t -\inner{t^3}{\frac{1}{\sqrt{2}}} \cdot \frac{1}{\sqrt{2}}
    \\&= t^3 - \integral{\frac{45}{8}(t^5 - \frac{1}{3}t^3)} \cdot (t^2 - \frac{1}{3}) - \integral{\frac{3}{2}t^4} \cdot t - \integral{\frac{1}{2}t^3}
    \\&= t^3 - \frac{45}{8}\brackets{\frac{1}{6}t^6 - \frac{1}{12}t^4} \cdot (t^2 - \frac{1}{3}) - \brackets{\frac{3}{10}t^5} \cdot t - \brackets{\frac{1}{8}t^4}
    \\&= t^3 -\frac{3}{5}t
\end{align*}
\begin{align*}
    ||t^3 - \inner{t^3}{\sqrt{\frac{45}{8}}(t^2 - \frac{1}{3})} \cdot \sqrt{\frac{45}{8}}(t^2 - \frac{1}{3}) &- \inner{t^3}{\sqrt{\frac{3}{2}}t} \cdot \sqrt{\frac{3}{2}}t -\inner{t^3}{\frac{1}{\sqrt{2}}} \cdot \frac{1}{\sqrt{2}}||
    \\&= ||t^3 -\frac{3}{5}t||\\
    \\&= \sqrt{\integral{t^6-\frac{6}{5}t^4+\frac{9}{25}t^2}}
    \\&= \sqrt{\brackets{\frac{1}{7}t^7 - \frac{6}{25}t^5 + \frac{3}{25}t^3}}
    \\&= \sqrt{\frac{8}{175}}
\end{align*}    
\begin{align*}
    f_3
    &= \frac{t^3 - \inner{t^3}{\sqrt{\frac{45}{8}}(t^2 - \frac{1}{3})} \cdot \sqrt{\frac{45}{8}}(t^2 - \frac{1}{3}) - \inner{t^3}{\sqrt{\frac{3}{2}}t} \cdot \sqrt{\frac{3}{2}}t -\inner{t^3}{\frac{1}{\sqrt{2}}} \cdot \frac{1}{\sqrt{2}}}{||t^3 - \inner{t^3}{\sqrt{\frac{45}{8}}(t^2 - \frac{1}{3})} \cdot \sqrt{\frac{45}{8}}(t^2 - \frac{1}{3}) - \inner{t^3}{\sqrt{\frac{3}{2}}t} \cdot \sqrt{\frac{3}{2}}t -\inner{t^3}{\frac{1}{\sqrt{2}}} \cdot \frac{1}{\sqrt{2}}||}\\
    &= \frac{t^3-\frac{3}{5}t}{\sqrt{\frac{8}{175}}}\\
    &= \sqrt{\frac{175}{8}}(t^3-\frac{3}{5}t)
\end{align*}
Therefore, a orthonormal basis for $V_3$ is 
$(\frac{1}{\sqrt{2}}, \sqrt{\frac{3}{2}}t, \sqrt{\frac{45}{8}}(t^2 - \frac{1}{3}), \sqrt{\frac{175}{8}}(t^3-\frac{3}{5}t))$
