% \newcommand{\integral}[1]{\int_{-1}^{1} #1 \,dt}
% \newcommand{\brackets}[1]{\left[ #1 \right]_{-1}^{1}}
%\frac{1}{2^{n+m}n!m!}
\section{Legendre Polynomial}
\begin{proof}$\inner{P_n(t)}{P_m(t)} = 0$ for $n \neq m$\gap

    Let $n < m$ let
    \[
        u = \frac{d^n}{dt^n} (t^2 - 1)^n \quad
        du = \frac{d^{n+1}}{dt^{n+1}} (t^2 - 1)^n dt 
    \]
    \[
        v = \frac{d^{m-1}}{dt^{m-1}} (t^2 - 1)^m \quad
        dv = \frac{d^m}{dt^m} (t^2 - 1)^m dt
    \]

    Because of the chain rule, any derivative of $(t^2 - 1)^m$ up to the $m-1$th derivative
    will have $t^2 - 1$ as a term and equal zero when $t = -1, 1$.
    Since the largest power in $(t^2-1)^n$ is $t^{2n}$ and $n+m > 2n$,
    the $m+n$th derivative of $(t^2-1)^n$ must equal zero.
    We have that
    \begin{align*}
        \integral{\frac{d^n}{dt^n} (t^2 - 1)^n \frac{d^m}{dt^m} (t^2 - 1)^m}
        &= \brackets{\frac{d^n}{dt^n} (t^2 - 1)^n \frac{d^{m-1}}{dt^{m-1}} (t^2 - 1)^m} - \integral{\frac{d^{m-1}}{dt^{m-1}} (t^2 - 1)^m \frac{d^{n+1}}{dt^{n+1}} (t^2 - 1)^n}\\
        &= -\integral{\frac{d^{n+1}}{dt^{n+1}} (t^2 - 1)^n \frac{d^{m-1}}{dt^{m-1}} (t^2 - 1)^m}\\
        &= \integral{\frac{d^{n+2}}{dt^{n+2}} (t^2 - 1)^n \frac{d^{m-2}}{dt^{m-2}} (t^2 - 1)^m}\\
        &\qquad \vdots\\
        &= \integral{\frac{d^{n+m}}{dt^{n+m}} (t^2 - 1)^n \frac{d^{0}}{dt^{0}} (t^2 - 1)^m}\\
        &= \integral{(t^2 - 1)^m \frac{d^{n+m}}{dt^{n+m}} (t^2 - 1)^n}\\
        &= 0
    \end{align*}\gap

    
    Since the inner product is commutative, and the inner product equals
    \[
        \inner{P_n(t)}{P_m(t)}
        =\frac{1}{2^{n+m}n!m!} \integral{\frac{d^n}{dt^n} (t^2 - 1)^n \frac{d^m}{dt^m} (t^2 - 1)^m}
        = 0
    \]
    we have that $\inner{P_n(t)}{P_m(t)} = 0$ for $n \neq m$.

  
\end{proof}
