\subsection*{Section 9.7}
\textbf{Problem 1}
The characteristic polynomial is 
\[
    (6-\lambda)(3-\lambda) - 4
    = 14 - 9\lambda + \lambda^2
    = (\lambda - 2)(\lambda-7)
\]
The eigenvalues are $\lambda_1 = 2$ and $\lambda_2 = 7$

The eigenvector for $\lambda_1$ is 
\[
    \begin{bmatrix}
        4 & 1 \\
        4 & 1
    \end{bmatrix} x = 0
    \implies x = 
    \begin{bmatrix}
        1 \\ -1
    \end{bmatrix}
\]
The eigenvector for $\lambda_2$ is 
\[
    \begin{bmatrix}
        -1 & 1 \\
        4 & -4
    \end{bmatrix} x = 0
    \implies x = 
    \begin{bmatrix}
        1 \\ 1
    \end{bmatrix}
\]
The homogenous solution is in the form 
\[
    y = c_1e^{2t} 
    \begin{bmatrix}
        1 \\ -1
    \end{bmatrix} +
    c_2e^{7t}
    \begin{bmatrix}
        1 \\ 1
    \end{bmatrix}
\]
Solving the system of equations,
\[
    \begin{bmatrix}
        0 \\
        0
    \end{bmatrix} = 
    \begin{bmatrix}
        6 & 1 \\
        4 & 3
    \end{bmatrix}
    \begin{bmatrix}
        a_1 \\
        a_2
    \end{bmatrix} +
     \begin{bmatrix}
         -11 \\ -5
     \end{bmatrix}
\]
This has solution 
\[
    a = \begin{bmatrix}
        2 \\ -1
    \end{bmatrix}
\]
The final solution is 
\[
    y = c_1e^{2t} 
    \begin{bmatrix}
        1 \\ -1
    \end{bmatrix} +
    c_2e^{7t}
    \begin{bmatrix}
        1 \\ 1
    \end{bmatrix}
    +
    \begin{bmatrix}
        2 \\ -1
    \end{bmatrix}
\]

\textbf{Problem 2}
The characteristic polynomial is 
\[
    (1-\lambda)^2-4
    = -3 -2\lambda + \lambda^2
    = (\lambda+1)(\lambda -3)
\]
The eigenvalues are $\lambda_1 = -1$ and $\lambda_2 = 3$.

The eigenvector for $\lambda_1$ is 
\[
    \begin{bmatrix}
        2 & 1 \\
        4 & 2
    \end{bmatrix} x = 0
    \implies x = \begin{bmatrix}
        1 \\ -2
    \end{bmatrix}
\]
The eigenvector for $\lambda_2$ is 
\[
    \begin{bmatrix}
        -2 & 1 \\
        4 & -2
    \end{bmatrix} x = 0
    \implies x = \begin{bmatrix}
        1 \\ 2
    \end{bmatrix}
\]
The homogenous solution is in the form 
\[
    y = c_1e^{-t} 
    \begin{bmatrix}
        1 \\ -2
    \end{bmatrix} +
    c_2e^{3t}
    \begin{bmatrix}
        1 \\ 2
    \end{bmatrix}
\]
Solving the system of equations for the particular solution,
\[
    \begin{bmatrix}
        a_1 \\ a_2
    \end{bmatrix} = 
    \begin{bmatrix}
        1 & 1 \\
        4 & 1
    \end{bmatrix}
    \begin{bmatrix}
        a_1t + b_1 \\ a_2t + b_2
    \end{bmatrix} +
    \begin{bmatrix}
        -t-1 \\ -4t-2
    \end{bmatrix}
\]
This can be rewritten as 
\[
    \begin{bmatrix}
        0 \\ 0
    \end{bmatrix} = 
    t \begin{bmatrix}
        a_1 + a_2 - 1 \\
        4a_1 + a_2 - 4
    \end{bmatrix} +
    \begin{bmatrix}
        b_1 + b_2 - a_1 - 1 \\
        4b_1 + b_2 - a_2 - 2
    \end{bmatrix} 
\]
Having $a_1 = 1$ and $a_2 = 0$ solves the first system and 
having $b_1 = 0$ and $b_2 = 2$ solves the second system.
The final solution is 
\[
    y = c_1e^{-t} 
    \begin{bmatrix}
        1 \\ -2
    \end{bmatrix} +
    c_2e^{3t}
    \begin{bmatrix}
        1 \\ 2
    \end{bmatrix} +
    \begin{bmatrix}
        t \\ 2
    \end{bmatrix}
\]
\textbf{Problem 8}
The particular solution has form 
\[
    t^2a + tb + c
\]