\subsection*{Section 9.5}
\textbf{Problem 3}
The characteristic polynomial is 
\[
    \det(A-\lambda I) 
    = (1-\lambda)(4-\lambda) + 2
    = 6 - 5\lambda + \lambda^2
    = (\lambda - 2)(\lambda - 3)
\]
The eigenvalues values are $\lambda_1 = 2$, $\lambda_2 = 3$.

The eigenvector for $\lambda_1$ is
\[
    (A-\lambda_1 I)x_1 = 0
    \implies 
    \begin{bmatrix}
        -1 & -1 \\
        2 & 2
    \end{bmatrix} x_1 = 0
    \implies x_1 = 
    \begin{bmatrix}
        1 \\ -1
    \end{bmatrix}
\]
The eigenvector for $\lambda_2$ is
\[
    (A-\lambda_2 I)x_2 = 0
    \implies 
    \begin{bmatrix}
        -2 & -1 \\
        2 & 1
    \end{bmatrix} x_2 = 0
    \implies x_1 = 
    \begin{bmatrix}
        1 \\ -2
    \end{bmatrix}
\]
\textbf{Problem 9}
The characteristic polynomial is 
\[
    \det(A-\lambda I)
    = \lambda^2 + 1
\]
The eigenvalues are $\lambda_1 = -i$ and $\lambda_2 = i$.

The eigenvector for $\lambda_1$ is 
\[
    (A-\lambda_1 I)x_1 = 0
    \implies 
    \begin{bmatrix}
        i & -1 \\
        1 & i
    \end{bmatrix} x_1 = 0
    \implies x_1 = 
    \begin{bmatrix}
        1 \\ i
    \end{bmatrix}
\]
The eigenvector for $\lambda_2$ is 
\[
    (A-\lambda_2 I)x_2 = 0
    \implies 
    \begin{bmatrix}
        -i & -1 \\
        1 & -i
    \end{bmatrix} x_2 = 0
    \implies x_2 = 
    \begin{bmatrix}
        1 \\ -i
    \end{bmatrix}
\]
\textbf{Problem 11}
The characteristic polynomial is 
\[
    \det(A-\lambda)
    = (-1-\lambda)(3-\lambda) + \frac{15}{4}
    = \frac{3}{4} - 2\lambda + \lambda^2
    = (\lambda-\frac{1}{2})(\lambda-\frac{3}{2})
\]
The eigenvalues are $\lambda_1 = \frac{1}{2}$ and $\lambda_2 = \frac{3}{2}$

The eigenvector for $\lambda_1$ is 
\[
    (A-\lambda_1 I)x_1 = 0
    \implies 
    \begin{bmatrix}
        -\frac{3}{2} & \frac{3}{4} \\
        -5 & \frac{5}{2}
    \end{bmatrix} x_1 = 0
    \implies x_1 = 
    \begin{bmatrix}
        1 \\ 2
    \end{bmatrix}
\]
The eigenvector for $\lambda_2$ is
\[
    (A-\lambda_2 I)x_2 = 0
    \implies 
    \begin{bmatrix}
        -\frac{5}{2} & \frac{3}{4} \\
        -5 & \frac{3}{2}
    \end{bmatrix} x_2 = 0
    \implies x_2 = 
    \begin{bmatrix}
        3 \\ 10
    \end{bmatrix}
\]
The general solution is 
\[
    y = c_1e^\frac{t}{2}\begin{bmatrix} 1 \\ 2 \end{bmatrix} + 
    c_2e^\frac{3t}{2} \begin{bmatrix} 3 \\ 10 \end{bmatrix}
\]
\textbf{Problem 12}
The characteristic polynomial is 
\[
    \det(A-\lambda I)
    = (1-\lambda)^2 - 36
    = 35 - 2\lambda + \lambda^2
    = (\lambda + 5)(\lambda - 7)
\]
The eigenvalues are $\lambda_1 = -5$ and $7$

The eigenvector for $\lambda_1$ is 
\[
    (A-\lambda_1 I)x_1 = 0
    \implies 
    \begin{bmatrix}
        6 & 3 \\
        12 & 6
    \end{bmatrix} x_1 = 0
    \implies x_1 = 
    \begin{bmatrix}
        1 \\ -2
    \end{bmatrix}
\]
The eigenvector for $\lambda_2$ is 
\[
    (A-\lambda_2 I)x_2 = 0
    \implies 
    \begin{bmatrix}
        -6 & 3 \\
        12 & -6
    \end{bmatrix} x_2 = 0
    \implies x_2 = 
    \begin{bmatrix}
        1 \\ 2
    \end{bmatrix}
\]
The general solution is 
\[
    y = c_1e^{-5t} \begin{bmatrix} 1 \\ -2 \end{bmatrix} +
    c_2e^{7t} \begin{bmatrix} 1 \\ 2 \end{bmatrix}
\]
\textbf{Problem 18}
\begin{enumerate}
    \item The matrix multiplies $u_1$ by $-1$
    \[
        \begin{bmatrix}
            -2 & 1 \\
            1 & -2
        \end{bmatrix}
        \begin{bmatrix}
            1 \\ 1
        \end{bmatrix}
        = \begin{bmatrix}
            -1 \\ -1
        \end{bmatrix}
    \]
    The matrix multiplies $u_2$ by $-3$
    \[
        \begin{bmatrix}
            -2 & 1 \\
            1 & -2
        \end{bmatrix}
        \begin{bmatrix}
            1 \\ -1
        \end{bmatrix}
        = \begin{bmatrix}
            -3 \\ 3
        \end{bmatrix}
    \]
    \item The equation is \[
        y = e^{-t} \begin{bmatrix}
            1 \\ 1
        \end{bmatrix}
    \]
    The equation starts at $(1,1)$ at $t=0$ and approaches 
    the origin as $t \to \infty$ in a straight line.
    \item The equation is \[
        y = e^{-3t} \begin{bmatrix}
            -1 \\ 1
        \end{bmatrix}
    \]
    The equation starts at $(-1,1)$ at $t=0$ and approaches 
    the origin as $t \to \infty$ in a straight line.
    \item The equation is \[
        y = e^{-t} \begin{bmatrix}
            1 \\ 1
        \end{bmatrix}
        +
        e^{-3t} \begin{bmatrix}
            -1 \\ 1
        \end{bmatrix}
    \]
    The equation starts at $(0, 2)$ at $t=0$ and approaches 
    the origin as $t \to \infty$ in a curve that goes rightward.
\end{enumerate}
\textbf{Problem 19}
The characteristic polynomial is 
\[
    \det(A-\lambda I)
    = (-1-\lambda)(1-\lambda) - 8
    = -9 + \lambda^2
    = (\lambda + 3)(\lambda - 3)
\]
The eigenvalues are $\lambda_1 = -3$ and $\lambda_2 = 3$.

The eigenvector for $\lambda_1$ is
\[
    (A-\lambda_1 I)x_1 = 0
    \implies 
    \begin{bmatrix}
        2 & 1 \\
        8 & 4
    \end{bmatrix} x_1 = 0
    \implies x_1 = 
    \begin{bmatrix}
        1 \\ -2
    \end{bmatrix}
\]
The eigenvector for $\lambda_2$ is 
\[
    (A-\lambda_2 I)x_2 = 0
    \implies 
    \begin{bmatrix}
        -4 & 1 \\
        8 & -2
    \end{bmatrix} x_2 = 0
    \implies x_2 = 
    \begin{bmatrix}
        1 \\ 4
    \end{bmatrix}
\]
The fundamental matrix is
\[
    \begin{bmatrix}
        e^{-3t} & e^{3t} \\
        -2e^{-3t} & 4e^{3t}
    \end{bmatrix}
\]
\textbf{Problem 20}
The characteristic polynomial is 
\[
    \det(A-\lambda I)
    = (5-\lambda)(-\lambda) + 4
    = \lambda^2 - 5\lambda + 4
    = (\lambda-1)(\lambda-4)
\]
The eigenvalues are $\lambda_1 = 1$ and $\lambda_2 = 4$.

The eigenvector for $\lambda_1$ is 
\[
    (A-\lambda_1 I)x_1 = 0
    \implies 
    \begin{bmatrix}
        4 & 4 \\
        -1 & -1
    \end{bmatrix} x_1 = 0
    \implies x_1 = 
    \begin{bmatrix}
        1 \\ -1
    \end{bmatrix}
\]
The eigenvector for $\lambda_2$ is 
\[
    (A-\lambda_2 I)x_2 = 0
    \implies 
    \begin{bmatrix}
        1 & 4 \\
        -1 & -4
    \end{bmatrix} x_2 = 0
    \implies x_2 = 
    \begin{bmatrix}
        4 \\ -1
    \end{bmatrix}
\]
The fundamental matrix is 
\[
    \begin{bmatrix}
        e^t & 4e^{4t} \\
        -e^t & -e^{4t}
    \end{bmatrix}
\]