\subsection*{Section 9.6}
\textbf{Problem 1}
The characteristic equation is 
\[
    \det(A-\lambda I)
    = (2-\lambda)(-2-\lambda) + 8
    = 4 + \lambda^2
\]
The eigenvalues are $\lambda_1 = -2i$ and $\lambda_2 = 2i$.

The eigenvector of $\lambda_2$ is 
\[
    (A-\lambda_2I)x=0 \implies 
    \begin{bmatrix}
        2-2i & -4 \\
        2 & -2-2i
    \end{bmatrix} x = 0 \implies
    x = 
    \begin{bmatrix}
        1+i \\ 1
    \end{bmatrix} = 
    \begin{bmatrix}
        1 \\ 1
    \end{bmatrix} +
    i
    \begin{bmatrix}
        1 \\ 0
    \end{bmatrix} 
\]
The general solution is 
\[
    y = c_1\left(\cos 2t \begin{bmatrix} 1 \\ 1 \end{bmatrix} 
          - \sin 2t \begin{bmatrix} 1 \\ 0 \end{bmatrix}\right) +
        c_2\left(\sin 2t \begin{bmatrix} 1 \\ 1 \end{bmatrix} 
          + \cos 2t \begin{bmatrix} 1 \\ 0 \end{bmatrix}\right) 
\]
This can be rewritten as 
\[
    y = c_1 
    \begin{bmatrix}
        \cos 2t - \sin 2t \\
        \cos 2t
    \end{bmatrix} +
    c_2 
    \begin{bmatrix}
        \sin 2t + \cos 2t \\
        \sin 2t
    \end{bmatrix}
\]
\textbf{Problem 2}
The characteristic polynomial is 
\[
    (-2-\lambda)(2-\lambda) + 5
    = 1 +\lambda^2
\]
The eigenvalues are $\pm i$
The eigenvector is 
\[
    (A-\lambda I)x=0 \implies 
    \begin{bmatrix}
        -2-i & -5 \\
        1 & 2-i
    \end{bmatrix} x = 0 \implies
    x = 
    \begin{bmatrix}
        i-2 \\ 1
    \end{bmatrix} = 
    \begin{bmatrix}
        -2 \\ 1
    \end{bmatrix} +
    i
    \begin{bmatrix}
        1 \\ 0
    \end{bmatrix} 
\]
The general solution is 
\[
    y = c_1\left(\cos t \begin{bmatrix} -2 \\ 1 \end{bmatrix} 
          - \sin t \begin{bmatrix} 1 \\ 0 \end{bmatrix}\right) +
        c_2\left(\sin t \begin{bmatrix} -2 \\ 1 \end{bmatrix} 
          + \cos t \begin{bmatrix} 1 \\ 0 \end{bmatrix}\right) 
\]
This can be rewritten as 
\[
    y = c_1 
    \begin{bmatrix}
        -2\cos t - \sin t \\
        \cos t
    \end{bmatrix} +
    c_2 
    \begin{bmatrix}
        -2\sin t + \cos t \\
        \sin t
    \end{bmatrix}
\]
\textbf{Problem 5}
The characteristic polynomial is 
\[
    (-1-\lambda)^2 + 16
    = 17 + 2\lambda + \lambda^2
    \implies \lambda = 
    \frac{-2 \pm \sqrt{4-68}}{2} =
    -1 \pm 4i
\]
The eigenvector is 
\[
    (A-\lambda I)x=0 \implies 
    \begin{bmatrix}
        -4i & -2 \\
        8 & -4i
    \end{bmatrix} x = 0 \implies
    x = 
    \begin{bmatrix}
        1 \\ -2i
    \end{bmatrix} = 
\]
The general solution is
\[
    y = c_1\left(e^{-t}\cos 4t \begin{bmatrix} 1 \\ 0 \end{bmatrix} 
          - e^{-t}\sin 4t \begin{bmatrix} 0 \\ -2 \end{bmatrix}\right) +
        c_2\left(e^{-t}\sin 4t \begin{bmatrix} 1 \\ 0 \end{bmatrix} 
          + e^{-t}\cos 4t \begin{bmatrix} 0 \\ -2 \end{bmatrix}\right) 
\]
The fundamental matrix is 
\[
    \begin{bmatrix}
        e^{-t}\cos 4t & e^{-t}\sin 4t \\
        2e^{-t}\sin 4t & -2e^{-t}\cos 4t
    \end{bmatrix}
\]
\textbf{Problem 6}
The characteristic polynomial is 
\[
    (-2-\lambda)(2-\lambda) + 8
    = 4 + \lambda^2
\]
The eigenvalues are $\pm 2i$
The eigenvector is 
\[
    (A-\lambda I)x=0 \implies 
    \begin{bmatrix}
        -2-2i & -2 \\
        4 & 2-2i
    \end{bmatrix} x = 0 \implies
    x = 
    \begin{bmatrix}
        1 \\ -1-i
    \end{bmatrix}
\]
The general solution is 
\[
    y = c_1\left(\cos 2t \begin{bmatrix} 1 \\ -1 \end{bmatrix} 
          - \sin 2t \begin{bmatrix} 0 \\ -1 \end{bmatrix}\right) +
        c_2\left(\sin 2t \begin{bmatrix} 1 \\ -1 \end{bmatrix} 
          + \cos 2t \begin{bmatrix} 0 \\ -1 \end{bmatrix}\right) 
\]
The fundamental matrix is 
\[
    \begin{bmatrix}
        \cos 2t & \sin 2t \\
        -\cos 2t + \sin 2t & -\sin 2t -\cos 2t
    \end{bmatrix}
\]
\textbf{Problem 13}
The characteristic equation is
\[
    (-3-\lambda)(-1-\lambda) + 2
    = 5 + 4\lambda + \lambda^2
    \implies \lambda =
    \frac{-4 \pm \sqrt{16-20}}{2} =
    -2 \pm i
\]
The eigenvalues are $-2 \pm i$ 

The eigenvector is
\[
    \begin{bmatrix}
        -1 - i & -1 \\
        2 & 1-i
    \end{bmatrix} x = 0
    \implies x = 
    \begin{bmatrix}
        1 \\ -1-i
    \end{bmatrix}
\]
The general solution is 
\[
    y = c_1\left(e^{-2t}\cos t \begin{bmatrix} 1 \\ -1 \end{bmatrix} 
          - e^{-2t}\sin t \begin{bmatrix} 0 \\ -1 \end{bmatrix}\right) +
        c_2\left(e^{-2t}\sin t \begin{bmatrix} 1 \\ -1 \end{bmatrix} 
          + e^{-2t}\cos t \begin{bmatrix} 0 \\ -1 \end{bmatrix}\right) 
\]
This can be rewritten as 
\[
    y = c_1
    \begin{bmatrix}
        e^{-2t}\cos t \\
        -e^{-2t}\cos t + e^{-2t}\sin t
    \end{bmatrix} + 
    c_2
    \begin{bmatrix}
        e^{-2t}\sin t \\
        -e^{-2t}\sin t - e^{-2t}\cos t
    \end{bmatrix}
\]
Solving out for the constants yields 
\begin{enumerate}
    \item \[
        x(0) = \begin{bmatrix}
            c_1 \\
            -c_1 -c_2
        \end{bmatrix}
    \]
    This means that $c_1 = -1$ and $c_2 = 1$.
    The solution is 
    \[
        \begin{bmatrix}
            e^{-2t}\sin t - e^{-2t}\cos t \\
            -2e^{-2t}\sin t
        \end{bmatrix}
    \]
    \item \[
        x(\pi) = e^{-2\pi}\begin{bmatrix}
            -c_1 \\
            c_1 -c_2
        \end{bmatrix}
    \]
    This means that $c_1 = -e^{2\pi}$ and $c_2 = 0$.
    The solution is 
    \[
        \begin{bmatrix}
            e^{-2t+2\pi} \cos t\\
            -e^{-2t+2\pi} \cos t + e^{-2t+2\pi} \sin t
        \end{bmatrix}
    \]
    \item \[
        x(-2\pi) = e^{4\pi}\begin{bmatrix}
            c_1 \\
            -c_1 -c_2
        \end{bmatrix}
    \]
    This means that $c_1 = 2e^{-4\pi}$ and $c_2 = -3e^{-4\pi}$.
    The solution is 
    \[
        \begin{bmatrix}
            e^{-2t+4\pi}(2\cos t - 3 \sin t) \\
            e^{-2t+4\pi}(\cos t + 5\sin t)
        \end{bmatrix}
    \]
    \item \[
        x(\pi/2) = e^{-\pi}\begin{bmatrix}
            c_2 \\
            c_1 -c_2
        \end{bmatrix} 
    \]
    This means that $c_1 = e^\pi$ and $c_2 = 0$
    The solution is 
    \[ 
        \begin{bmatrix}
            e^{\pi - 2t}\cos t \\
            e^{\pi - 2t}(\sin t - \cos t)
        \end{bmatrix}
    \]
\end{enumerate}