\subsection*{Section 1.2}
\textbf{Problem 1}
\begin{enumerate}
    \item Show that $\phi(x) = x^2$ is a solution to 
        \[
            x\der{y}{x} = 2y
        \]
    \item Show that $\phi(x) = e^x-x$ is a solution to 
        \[
            \der{y}{x} + y^2 = e^{2x} + (1-2x)e^x + x^2 -1
        \]
    \item Show that $\phi(x) = x^2 - x\inv$ is a solution to
        \[
            x^2 \der[2]{y}{x} = 2y
        \]
\end{enumerate}
\solution
\begin{enumerate}
    \item Substituting $\phi(x)$ in for $y$ yields an equation 
        that is true for all $x \in (-\infty, \infty)$.
        \[
            x\der{y}{x} = 2y
            \implies x(2x) = 2(x^2)
            \implies 2x^2 = 2x^2
        \]
    \item Substituting $\phi(x)$ in for $y$ yields an equation
        that is true for all $x \in (-\infty, \infty)$.
        \begin{align*}
            \der{y}{x} + y^2 = e^{2x} + (1-2x)e^x + x^2 -1
            &\implies (e^x-1) + (e^x-x)^2 = e^{2x} + (1-2x)e^x + x^2 -1 \\
            &\implies (e^x-1) + (e^x-x)^2 = (e^x-x)^2 + e^x - 1 \\ 
            &\implies (e^x-1) + (e^x-x)^2 = (e^x-1) + (e^x-x)^2
        \end{align*}
    \item Substituting $\phi(x)$ in for $y$ yields an equation
        that is true for all $x \in (0, \infty)$.
        \begin{align*}
            x^2 \der[2]{y}{x} = 2y
            &\implies x^2 (2- 2x^{-3}) = 2(x^2-x\inv) \\
            &\implies 2x^2 - 2x\inv = 2x^2-2x\inv
        \end{align*}
\end{enumerate}
\textbf{Problem 4}

Determine if $x = 2\cos t - 3\sin t$ is a solution to $x''+ x = 0$ \\
\solution
It is a solution since 
\begin{align*}
    x''+ x = 0
    &\implies (-2\cos t + 3\sin t) + (2\cos t - 3\sin t) = 0 \\
    &\implies 0 = 0
\end{align*}
\textbf{Problem 10}

Determine if $y-\ln(y) = x^2+1$ is an implicit solution to 
$\der{y}{x} = \frac{2xy}{y-1}$ \\
\solution 
It is a solution since
\begin{align*}
    y-\ln(y) = x^2+1
    &\implies \der{y}{x} - \frac{1}{y}\der{y}{x} = 2x \\
    &\implies \der{y}{x} (1-\frac{1}{y}) = 2x \\ 
    &\implies \der{y}{x} (\frac{y-1}{y}) = 2x \\ 
    &\implies \der{y}{x} = \frac{2xy}{y-1}
\end{align*}
\textbf{Problem 22}

Verify that $\phi(x) = c_1e^x + c_2e^{-2x}$
is a solution to 
\[
    \der[2]{y}{x} + \der{y}{x} - 2y = 0
\]
and find $c_1$ and $c_2$ that satisfies
\begin{enumerate}
    \item $y(0) = 2$, $y'(0) = 1$
    \item $y(1) = 1$, $y'(1) = 0$
\end{enumerate} 
\solution 
Substituting in $\phi$ yields 
\begin{align*}
    \der[2]{y}{x} + \der{y}{x} - 2y = 0
    &\implies (c_1e^x + 4c_2e^{-2x}) + (c_1e^x - 2c_2e^{-2x}) - 2(c_1e^x + c_2e^{-2x}) = 0 \\
    &\implies 0 = 0
\end{align*}
\begin{enumerate}
    \item 
        \[
            \phi(0) = 2 
            \implies c_1e^0 + c_2e^0 = 2
            \implies c_1 + c_2 = 2
        \]
        \[
            \phi'(0) = 1
            \implies c_1e^0 - 2c_2e^0 = 1
            \implies c_1 - 2c_2 = 1
        \]
        Solving this system of equations yields 
        $c_1 = \frac{5}{3}$ and $c_2 = \frac{1}{3}$.
    \item 
        \[
            \phi(1) = 1
            \implies c_1e^1 + c_2e^{-2} = 1
            \implies ec_1 + e^{-2}c_2 = 1
        \]
        \[
            \phi'(1) = 0
            \implies c_1e^1 - 2c_2e^{-2} = 0
            \implies ec_1 - 2 e^{-2}c_2 = 0
        \]
        Solving this system of equations yields 
        $c_1 = \frac{2}{3e}$ and $c_2 = \frac{e^2}{3}$.
\end{enumerate}
\textbf{Problem 24}

Does $\der{y}{t} - ty = \sin^2 t$ with $y(\pi)=5$
have a unique solution? \\
\solution
$f(t,y) = ty + \sin^2 t$ is always continuous and 
$\pder{f}{y} = t$ is also always continuous so 
the differential equation has a unique solution.

\textbf{Problem 26}

Does $\der{x}{t} + \cos x = \sin t$ with $x(\pi) = 0$
have a unique solution? \\
\solution 
$f(t,x) = \sin t-\cos x$ is always continuous and 
$\pder{f}{x} = \sin x$ is also always continuous so 
the differential equation has a unique solution.

\textbf{Problem 28}

Does $\der{y}{x} = 3x - \sqrt[3]{y-1}$ with $y(2) = 1$
have a unique solution? \\
\solution 
$f(x, y) = 3x - \sqrt[3]{y-1}$ is always continuous but
$\pder{f}{y} = -\frac{1}{3}(y-1)^{-\frac{2}{3}}$ 
is not continuous for $y_0 = 1$ so 
the theorem does not apply.

\newpage 