\section{Determinants and block matrices}
\begin{proof} If the bottom left $m \times n$ block is zeros,
    the determinant is equal to $\det(A) \cdot \det(C)$. \gap

    \textbf{Base Case: }
    When 
    $\begin{bmatrix}
        A & B\\
        0 & C
    \end{bmatrix}$ is a $2 \times 2$ matrix,
    $\det(A) = AC - B \cdot 0 = AC = \det(A) \cdot \det(C)$.
    
    \textbf{Inductive Step: }
    Assume that  
    $\begin{bmatrix}
        A & B\\
        0 & C
    \end{bmatrix}
    = \det(A) \cdot \det(C)$
    for when $A$ is $m \times m$ and $C$ is $n-1 \times n-1$.
    For any row index $i$, the cofactor formula says that
    \[ \det(M) = \sum_{j=1}^{m+n} (-1)^{i+j} m_{ij} \det(M_{ij}) \]

    Let $i = m+n$. In the cofactor formula, 
    the first $n$ terms are equal to zero since $m_{ij} = 0$.
    When $n < j \leq m+n$, the term is equal to 
    $(-1)^{i+j} m_{ij} \det(M_{ij})$. 
    By our assumption for when $C$ is $n-1 \times n-1$,
    $\det(M_{ij}) = \det(A) \cdot \det(C_{ij})$.
    Therefore,
    \begin{align}
        \det(M) 
        &= \sum_{j=n+1}^{m+n} (-1)^{i+j} m_{ij} \det(A) \cdot \det(C_{ij}) 
        &= \det(A) \sum_{j=n+1}^{m+n} (-1)^{i+j} m_{ij} \det(C_{ij}) 
        &= \det(A) \cdot \det(C)
    \end{align}

    This completes the inductive step, so
    $\det(M) = \det(A) \cdot \det(C)$

\end{proof}