\subsection*{Section 9.3}
\textbf{Problem 9}
\begin{align*}
    \begin{bmatrix}
        2 & 1 & 1 & 0 \\
        -1 & 4 & 0 & 1
    \end{bmatrix}
    &\implies \begin{bmatrix}
        2 & 1 & 1 & 0 \\
        0 & \frac{9}{2} & \frac{1}{2} & 1
    \end{bmatrix} \\
    &\implies \begin{bmatrix}
        2 & 0 & \frac{8}{9} & -\frac{2}{9} \\
        0 & \frac{9}{2} & \frac{1}{2} & 1
    \end{bmatrix} \\
    &\implies \begin{bmatrix}
        1 & 0 & \frac{4}{9} & -\frac{1}{9} \\
        0 & 1 & \frac{1}{9} & \frac{2}{9}
    \end{bmatrix} 
\end{align*}
This aligns with the formula 
\[
    \frac{1}{ad-bc}
    \begin{bmatrix}
        d & -b \\
        -c & a
    \end{bmatrix}
    = \frac{1}{9}
    \begin{bmatrix}
        4 & -1 \\
        1 & 2
    \end{bmatrix}
\]
\textbf{Problem 17}
Using the equation for the inverse of a $2 \times 2$,
\[
    \frac{1}{ad-bc}
    \begin{bmatrix}
        d & -b \\
        -c & a
    \end{bmatrix}
    = \frac{1}{3e^5}
    \begin{bmatrix}
        4e^{4t} & -e^{4t} \\
        -e^t & e^t
    \end{bmatrix}
    = \frac{1}{3}
    \begin{bmatrix}
        4e^{-t} & -e^{-t} \\
        -e^{-4t} & e^{-4t}
    \end{bmatrix}
\]
\textbf{Problem 18}
Using the equation for the inverse of a $2 \times 2$,
\[
    \frac{1}{ad-bc}
    \begin{bmatrix}
        d & -b \\
        -c & a
    \end{bmatrix}
    = \frac{1}{-2\sin^2 2t - 2\cos^2 2t}
    \begin{bmatrix}
        -2\sin 2t & -\cos 2t \\
        -2\cos 2t & \sin 2t
    \end{bmatrix}
    = 
    \begin{bmatrix}
        \sin 2t & \frac{1}{2}\cos 2t \\
        \cos 2t & -\frac{1}{2}\sin 2t
    \end{bmatrix}
\]
\textbf{Problem 22}
\[
    ad-bc = 24-24 = 0
\]
\textbf{Problem 27}
\[
    \det(A-rI)
    = (1-r)(4-r) +2
    = 6 - 5r + r^2 
    = (r-2)(r-3)
    \implies r=2,3
\]
\textbf{Problem 28}
\[
    \det(A-rI)
    = (3-r)(4-r) - 6
    = 6 - 7r + r^2 
    = (r-1)(r-6)
    \implies r=1,6
\]
\textbf{Problem 31}
\[
    x' =
    \begin{bmatrix}
        3e^{3t} \\  6e^{3t} \\ -3e^{3t}
    \end{bmatrix}
\]

\textbf{Problem 35}
\[
    x' =
    \begin{bmatrix}
        3e^{3t} \\  6e^{3t} 
    \end{bmatrix}
\]
\[
    Ax =
    \begin{bmatrix}
        e^{3t} + 2e^{3t} \\  
        -2e^{3t} + 8e^{3t}
    \end{bmatrix} =
    \begin{bmatrix}
        3e^{3t} \\  6e^{3t} 
    \end{bmatrix}
\]