\subsection*{Section 7.3}
\textbf{Problem 3}
    For $s>6$
    \begin{align*}
        \mathscr{L}(e^{-t}\cos 3t + e^{6t} - 1)
        &= \mathscr{L}(e^{-t}\cos 3t) + \mathscr{L}(e^{6t}) - \mathscr{L}(1) \\
        &= \frac{s+1}{(s+1)^2+9} + \frac{1}{s-6} - \frac{1}{s}
    \end{align*}
\textbf{Problem 7}
    For $s>0$
    \begin{align*}
        \mathscr{L}((t-1)^4)
        &= \mathscr{L}(t^4-4t^3+6t^2-4t+1) \\
        &= \frac{24}{s^5} - \frac{24}{s^4} + \frac{12}{s^3}
            - \frac{4}{s^2} + \frac{1}{s}
    \end{align*}
\textbf{Problem 12}
    For $s>0$
    \begin{align*}
        \mathscr{L}(\sin 3t \cos 3t)
        &= \frac{1}{2} \mathscr{L}(\sin 6t) \\
        &= \frac{3}{s^2+36}
    \end{align*}
\textbf{Problem 16}
    For $s>0$
    \begin{align*}
        \mathscr{L}(t\sin^2 t)
        &= \frac{1}{2}\mathscr{L}(t - t\cos 2t) \\
        &= \frac{1}{2s^2} + \frac{d}{ds}(\frac{s}{s^2+4}) \\
        &= \frac{1}{2s^2} + \frac{4-s^2}{2(s^2+4)^2} \\
    \end{align*}
\textbf{Problem 17}
    For $s>0$
    \begin{align*}
        \mathscr{L}(\sin 2t \sin 5t)
        &= \frac{1}{2}\mathscr{L}((\cos 3t - \cos 7t)) \\
        &= \frac{s}{2(s^2+9)} - \frac{s}{2(s^2+49)}
    \end{align*}
\textbf{Problem 21}
    Substituting in $s-a$ yields
    \[
        \mathscr{L}(e^{at}f(t))(s) 
        = \frac{s-a}{((s-a)^2 + b^2)}
    \]
\textbf{Problem 26}

    For $t \geq T$, $|f(t)| \leq Me^{\alpha t}$.
    For $0 \leq t < T$, the function is bounded since 
    since each piecewise function is continuous and the endpoints have limits.
    If the upperbound of $0 \leq t < T$ is $N$, 
    then $|f(t)| \leq Ke^{\alpha t}$ where $k = \max \{M, N\}$. \\

    Since this function is bounded by $Ke^{\alpha t}$
    \begin{align*}
        \lim_{s \to \infty }|\mathscr{L}\{f(t)\}(s)|
        &\leq \lim_{s \to \infty } \int_0^\infty Ke^{\alpha t}e^{-st} \\
        &= \lim_{s \to \infty } \frac{K}{s-\alpha} \\
        &= 0
    \end{align*}
\textbf{Problem 31}
    Using the definition,
    \[
        \mathscr{L}\{g\}(s)
        = \int_c^\infty e^{-st}f(t-c) \,dt 
        = \int_0^\infty e^{-st-cs}f(t) \,dt 
        = e^{-cs } \mathscr{L}\{f\}(s) 
    \]