\subsection*{Section 7.2}
\textbf{Problem 4}
    For $s > 3$
    \begin{align*}
        F(s) 
        &= \int_0^{\infty} e^{-st}f(t) \,dt \\
        &= \int_0^{\infty} te^{(3-s)t} \,dt \\
        &= \lim_{N \to \infty} \left[
            \left(\frac{t}{3-s} - \frac{1}{(3-s)^2}\right)e^{(3-s)t}
        \right]_0^N \\
        &= \lim_{N \to \infty} \left[
            \left(\frac{N}{3-s} - \frac{1}{(3-s)^2}\right)e^{(3-s)N}
        \right]+ \frac{1}{(3-s)^2} \\
        &= \lim_{N \to \infty} \left[
            \frac{1}{-(3-s)^2e^{-(3-s)N}} 
        \right] + \frac{1}{(3-s)^2} \\
        &= \frac{1}{(3-s)^2}
\end{align*}
\textbf{Problem 6}
    For $s > 0$,
    \begin{align*}
        F(s) 
        &= \int_0^{\infty} e^{-st}f(t) \,dt \\
        &= \int_0^{\infty} e^{-st}\cos bt \,dt \\
        &= \lim_{N \to \infty} \left[ 
            \frac{e^{-st}(-s\cos bt + b\sin bt)}{s^2+b^2}
        \right]_0^N \\
        &= \frac{s}{s^2+b^2}
    \end{align*}
\textbf{Problem 11}
    For all $s$
    \begin{align*}
        F(s) 
        &= \int_0^{\infty} e^{-st}f(t) \,dt \\
        &= \int_0^\pi e^{-st}\sin t \,dt 
            + \int_\pi^\infty 0 \,dt \\
        &= \left[
            -\frac{e^{-st}(s\sin(t)+\cos(t))}{s^2+1}
        \right]_0^\pi \\
        &= \frac{e^{-\pi s}}{s^2+1} + \frac{1}{s^2+1}
    \end{align*}
\textbf{Problem 17}
    For $s>3$
    \begin{align*}
        \mathscr{L}(e^3t\sin6t - t^3 + e^t)
        &= \mathscr{L}(e^3t\sin6t) - \mathscr{L}(t^3) + \mathscr{L}(e^t) \\
        &= \frac{6}{(s-3)^2+36}  - \frac{6}{s^4} + \frac{1}{s-1}
    \end{align*}
\textbf{Problem 18}
For $s>0$
\begin{align*}
    \mathscr{L}(t^4-t^2-t + \sin \sqrt{2}t)
    &= \mathscr{L}(t^4) - \mathscr{L}(t^2) - \mathscr{L}(t) + \mathscr{L}(\sin \sqrt{2}t) \\
    &= \frac{24}{s^5}  - \frac{2}{s^3} - \frac{1}{s^2} + \frac{\sqrt{2}}{s^2+2}
\end{align*}
\textbf{Problem 23}
    The graph is only piecewise continuous.
\textbf{Problem 28}
    The graph is continuous since 
    \[
        \lim_{t \to 0} \frac{\sin t}{t}
        = \lim_{t \to 0} \frac{\cos t}{1}
        = 1
    \]