\subsection*{Section 2.3}
\textbf{Problem 3}

Both

\textbf{Problem 4}

Linear

\textbf{Problem 12}

We have that 
$P(x) = 4$ and
$Q(x) = x^2e^{-4x}$.

The integrating factor is 
\[
    \mu(x)
    = e^{\int 4 \,dx}
    = e^{4x}
\]
Multiplying by the integrating factor gives 
\begin{align*}
    \der{y}{x} + 4y = x^2e^{-4x}
    &\implies \der{}{x} e^{4x}y = x^2 \\
    &\implies e^{4x}y = \frac{1}{3} x^3 + C \\ 
    &\implies y = \frac{1}{3} x^3e^{-4x} + Ce^{-4x}
\end{align*}

\textbf{Problem 14}

We have that 
$P(x) = \frac{3}{x}$ and 
$Q(x) = \frac{\sin x}{x^2} - 3x$.

The integrating factor is 
\[
    \mu(x)
    = e^{\int \frac{3}{x} \,dx}
    = e^{3\ln x}
    = x^3
\]
Multiplying by the integrating factor gives 
\begin{align*}
    \der{y}{x} + \frac{3}{x}y = \frac{\sin x}{x^2} - 3x
    &\implies \der{}{x} x^3y = x \sin x - 3x^4 \\ 
    &\implies x^3y = \sin x - x \cos x - \frac{3}{5}x^5 + C \\
    &\implies y = \frac{\sin x}{x^3} - \frac{\cos x}{x^2} - \frac{3}{5}x^2 + \frac{C}{x^3}
\end{align*}

\textbf{Problem 17}

We have that 
$P(x) = -\frac{1}{x}$ and
$Q(x) = xe^x$.

The integrating factor is 
\[
    \mu(x)
    = e^{\int -\frac{1}{x} \,dx}
    = \frac{1}{x}
\]
Multiplying by the integrating factor gives 
\begin{align*}
    \der{y}{x} - \frac{y}{x} = e^x
    &\implies \der{}{x} \frac{y}{x} = e^x \\
    &\implies \frac{y}{x} = e^x + C\\
    &\implies y = xe^x + Cx
\end{align*}

At $y(1) = e-1$,
\[
    y = xe^x + Cx
    \implies e-1 = e + C
    \implies C = -1
\]
Therefore the final solution is 
\[
    y = xe^x - x
\]
\textbf{Problem 20}

We have that 
$P(x) = \frac{3}{x}$ and 
$Q(x) = 3x-2$

The integrating factor is 
\[
    \mu(x)
    = e^{\int \frac{3}{x} \,dx}
    = x^3
\]
Multiplying by the integrating factor gives 
\begin{align*}
    \der{y}{x} + \frac{3}{x}y = 3x-2
    &\implies \der{}{x} x^3y = 3x^4-2x^3 \\
    &\implies x^3y = \frac{3}{5}x^5 - \frac{1}{2} x^4 + C \\
    &\implies y = \frac{3}{5}x^2 - \frac{1}{2} x + \frac{C}{x^3}
\end{align*}

At $y(1) = 1$,
\[
    y = \frac{3}{5}x^2 - \frac{1}{2} x + \frac{C}{x^3}
    \implies 1 = \frac{3}{5} - \frac{1}{2} + C
    \implies C = \frac{9}{10}
\]
Therefore the final solution is 
\[
    y = \frac{3}{5}x^2 - \frac{1}{2} x + \frac{9}{10x^3}
\]
\textbf{Problem 29}
Taking the reciprocal of both sides,
\[
    \der{y}{x} = \frac{1}{e^{4y}+2x}
    \implies \der{x}{y} = e^{4y}+2x
    \implies \der{x}{y} -2x = e^{4y}
\]

We have "switched" the roles of the variables, so 
$P(y) = -2$ and $Q(y) = e^{4y}$.
The integrating factor is 
\[
    \mu(y)
    = e^{\int -2 \,dy}
    = e^{-2y}
\]
Multiplying by the integrating factor gives 
\begin{align*}
    \der{x}{y} -2x = e^{4y}
    &\implies \der{}{y} e^{-2y}x = e^{2y} \\
    &\implies e^{-2y}x = \frac{1}{2}e^{2y} + C \\ 
    &\implies x = \frac{1}{2}e^{4y} + Ce^{2y}
\end{align*}


