\subsection*{Section 2.4}
\textbf{Problem 4}

Exact since both derivatives equal $xye^{xy}+x^{xy}$

\textbf{Problem 5}

Separable and linear

\textbf{Problem 6}

Exact since both derivatives equal $2y$

\textbf{Problem 10}

The equation is exact since both derivatives equal 1.
Thus, 
\[
    F(x,y) = \int 2x + y \,dx + g(y) = x^2 + xy + g(y)
\]
Taking the derivative with respect to $y$, 
\[
    x-2y = x + g'(y)
    \implies g'(y) = -2y
    \implies g(y) = -y^2
\]
Thus the general solution is
\[
    F(x,y) = x^2 + xy - y^2 = C
\]
\textbf{Problem 22}
The equation is exact so, 
\[
    F(x, y) 
    = \int ye^{xy}-\frac{1}{y} \,dx 
    = e^{xy} - \frac{x}{y} + g(y)
\]
Taking the derivative with respect to $y$,
\[
    xe^{xy}+\frac{x}{y^2} = xe^{xy} + \frac{x}{y^2} + g'(y)
    \implies  g'(y) = 0 
    \implies g(y) = C
\]
Thus the general solution is in form 
\[
    F(x, y) = e^{xy} - \frac{x}{y}  = C
\]
$C = e-1$ at $y(1) = 1$ so the solution is 
\[
    e^{xy} - \frac{x}{y}  = e-1
\]
\textbf{Problem 23}
The equation is exact so,
\[
    F(x, y)
    = \int e^ty + te^ty \,dt 
    = te^ty + g(y)
\]
Taking the derivative with respect to $y$,
\[
    te^t+2 = te^t + g'(y)
    \implies g'(y) = 2
    \implies g(y) = 2y+C
\]
Thus the general solution is in form 
\[
    te^ty + 2y = C
\]
$C = -2$ at $y(0) = -1$ so the solution is 
\[
    te^ty + 2y = -2
    \implies y = -\frac{2}{te^t+2}
\]
\textbf{Problem 26}
The equation is exact so,
\[
    F(x,y)
    = \int \tan y - 2 \,dx 
    = x\tan y - 2x + g(y)
\]
Taking the derivative with respect to $y$,
\[
    x\sec^2y + \frac{1}{y} = x\sec^2 y + g'(y)
    \implies g'(y) = \frac{1}{y}
    \implies g(y) = \ln y + C
\]
Thus the general solution is in form 
\[
    x\tan y - 2x + \ln y = C
\]
$C= 0$ at $y(0) = 1$ so the solution is 
\[
    x\tan y - 2x + \ln y = 0
\]
\textbf{Problem 29}
The equation is not exact since 
\[
    \pder{}{y} (y^2+2xy) = 2y+2x
\]
\[
    \pder{}{x} -x^2 = -2x
\]
Multiplying by $y^{-2}$ yields an exact solution since
\[
    \pder{}{y} (1+2\frac{x}{y}) = -2\frac{x}{y^2}
\]
\[
    \pder{}{x} (-\frac{x^2}{y^2}) = -2\frac{x}{y^2}
\]
Therefore,
\[
    F(x, y) 
    = \int (1+2\frac{x}{y}) \, dx 
    = x + \frac{x^2}{y} + g(y)
\]
Taking the derivative relative to $y$,
\[
    -\frac{x^2}{y^2} = - \frac{x^2}{y^2} + g'(y)
    \implies g'(y) = 0
    \implies g(y) = C
\]
The general solution is thus 
\[
    x + \frac{x^2}{y} = C
    \implies y = \frac{x^2}{C-x}
\]
The solution, $y=0$, was lost.